Can't prove the transitivity lemma

theories/Equiv/SimCompanion.v
@@ -34,12 +34,14 @@ Section Tower.
   Definition companion (R : A -> B -> C -> Prop) : A -> B -> C -> Prop :=
     fun a b c => forall S, T S -> R <3= S -> S a b c.
 
+  Notation "'㚘'" := companion (at level 0).
+
   Lemma T_companion x : T (companion x).
     repeat (eapply T_lim; intros).
     eauto.
   Qed.
 
-  Lemma compantion_monotone : monotone3 companion.
+  Lemma companion_monotone : monotone3 companion.
     hnf; intros. hnf; intros.
     eapply IN; eauto.
   Qed.
@@ -79,7 +81,7 @@ Section Tower.
     eapply H0. rewrite companion_img; eauto.
   Qed.
 
-  Lemma compantion_fold R
+  Lemma companion_fold R
     : monotone3 f -> f (companion R) <3= companion R.
   Proof.
     intro.
@@ -96,12 +98,59 @@ Section Tower.
     - isabsurd.
   Qed.
 
+  Section UptoLemma.
+    Variable g : (A -> B -> C -> Prop) -> (A -> B -> C -> Prop).
+    Hypothesis gP : monotone3 g.
+
+    Lemma upto :
+      (forall x, g (companion x) <3= companion x -> g (f (companion x)) <3= f (companion x)) ->
+      (forall x, g (companion x) <3= companion x).
+    Proof.
+      intros H1 H2.
+      eapply tower_ind.
+      - intros; hnf; intros; eauto.
+        hnf; eauto.
+      - intros; eauto.
+    Qed.
+
+    Lemma upto_below :
+      (forall x, g (companion x) <3= companion x) -> g <4= companion.
+    Proof.
+      intros H1 r; intros.
+      eapply H1. eapply gP; eauto.
+      eapply companion_inc.
+    Qed.
+
+    Lemma upto_char :
+      monotone3 f ->
+      g <4= companion ->
+      forall x, g (companion x) <3= companion x -> g (f (companion x)) <3= f (companion x).
+    Proof.
+      intros gM H1 r H2; intros.
+      eapply H1; eauto.
+      econstructor 1. eapply T_companion.
+    Qed.
+  End UptoLemma.
+
+    Lemma companion_unfold_r r
+    : monotone3 f -> companion r <3= f (companion r \3/ r).
+  Proof.
+    intros. hnf in PR. eapply PR.
+    - econstructor 1. admit.
+    - intros.
+      eapply H; try left; eauto.
+      (* eapply PR. *)
+
+  Admitted.
+
 End Tower.
+
+
 
 Definition simc {S} `{StateType S} {S'} `{StateType S'} r t (σ1:S) (σ2:S')
   := companion (@sim_gen S _ S' _) r t σ1 σ2.
 
-Theorem sim_simc {S} `{StateType S} {S'} `{StateType S'} r t (σ1:S) (σ2:S')
+Theorem simc_sim {S} `{StateType S} {S'} `{StateType S'} r t (σ1:S) (σ2:S')
   : simc bot3 t σ1 σ2 -> sim r t σ1 σ2.
 Proof.
   intros. revert t σ1 σ2 H1.
@@ -111,7 +160,7 @@ Proof.
 Qed.
 
 
-Theorem simc_sim {S} `{StateType S} {S'} `{StateType S'} r t (σ1:S) (σ2:S')
+Theorem sim_simc {S} `{StateType S} {S'} `{StateType S'} r t (σ1:S) (σ2:S')
   : sim bot3 t σ1 σ2 -> simc r t σ1 σ2.
 Proof.
   intros. revert t σ1 σ2 H1.
@@ -124,10 +173,362 @@ Proof.
     eapply H1. eauto.
 Qed.
 
-Lemma simc_trans {S} `{StateType S} {S'} `{StateType S'} r t
-       (σ1:S) (σ2:S) (σ3:S')
-  : simc bot3 t σ1 σ2
-    -> simc r t σ2 σ3
+Lemma simc_trans t {S1} `{StateType S1}
+      (σ1:S1) {S2} `{StateType S2} (σ2:S2) {S3} `{StateType S3} (σ3:S3)
+  : simc bot3 t σ1 σ2 -> simc bot3 t σ2 σ3 -> simc bot3 t σ1 σ3.
+Proof.
+  intros.
+  eapply sim_simc.
+  eapply sim_trans with (S2:=S2).
+  eapply simc_sim; eauto.
+  eapply simc_sim; eauto.
+Qed.
+
+Definition expc {S} `{StateType S} {S'} `{StateType S'}
+           (r:(simtype -> S -> S' -> Prop)) : simtype -> S -> S' -> Prop :=
+  fun t σ σ' => exists σ1 σ2, star2 step σ nil σ1 /\ star2 step σ' nil σ2 /\ r t σ1 σ2.
+
+Lemma expc_upto {S} `{StateType S} {S'} `{StateType S'}
+  : (forall r, @expc S _ S' _ (simc r) <3= simc r).
+Proof.
+  intros H1 H2.
+  eapply upto.
+  - unfold expc; hnf; intros.
+    destruct IN as [? [? [? [? ?]]]].
+    do  2eexists; split; eauto.
+  - unfold expc; intros.
+    destruct PR as [? [? [? [? ?]]]].
+    inv H6; zzsimpl; eauto 20.
+Qed.
+
+
+Lemma expc_simc {S} `{StateType S} {S'} `{StateType S'} (σ1 σ1':S) (σ2 σ2':S') t r
+  : simc r t σ1'  σ2'
+    -> star2 step σ1 nil σ1'
+    -> star2 step σ2 nil σ2'
+    -> simc r t σ1 σ2.
+Proof.
+  intros.
+  eapply expc_upto; hnf; eauto 20.
+Qed.
+
+
+Definition redc {S} `{StateType S} {S'} `{StateType S'}
+           (r:(simtype -> S -> S' -> Prop)) : simtype -> S -> S' -> Prop :=
+  fun t σ σ2 => exists σ1, star2 step σ1 nil σ (* /\ star2 step σ2 nil σ'*) /\ r t σ1 σ2.
+
+Lemma star2n_reach' X (R:X -> event -> X -> Prop) σ1 σ2a σ2b n n'
+: star2n R n σ1 nil σ2a
+  -> star2n R n' σ1 nil σ2b
+  -> internally_deterministic R
+  -> ((star2n R (n'-n) σ2a nil σ2b /\ n' > n) \/
+     (star2n R (n-n') σ2b nil σ2a /\ n > n')
+     \/ ( n' = n /\ σ2a = σ2b)).
+Proof.
+  intros Star1 Star2 IDet.
+  general induction Star1; eauto.
+  - orewrite (n' - 0 = n').
+    inv Star2; eauto.
+    left. rewrite H. split; eauto. omega.
+  - relsimpl. invc Star2; relsimpl; simpl; eauto.
+    + right. left. split. eapply (S_star2n _ _ H Star1). omega.
+    + edestruct IHStar1 as [?|[?|?]]; eauto; dcr.
+      * left. split; try omega. eauto.
+      * right. left. split; try omega. eauto.
+Qed.
+
+Lemma star2n_plus {S} `{StateType S} (σ σ':S) n
+  : star2n step n σ nil σ'
+    -> n > 0
+    -> plus2 step σ nil σ'.
+Proof.
+  intros. general induction H0.
+  - omega.
+  - destruct y, yl; isabsurd; simpl in *.
+    destruct n.
+    + inv H1. econstructor 1; eauto.
+    + econstructor 2; eauto. eapply IHstar2n; eauto.
+      omega.
+Qed.
+
+(*
+Lemma sim_reduction_closed_1 t {S} `{StateType S}
+      (σ1 σ1':S) {S'} `{StateType S'} (σ2:S') r
+  : simc r t σ1 σ2
+    -> star2 step σ1 nil σ1'
+    -> simc r t σ1' σ2.
+Proof.
+  intros Sim Star.
+  eapply star2_star2n in Star. destruct Star as[n StarN].
+  revert dependent r. revert σ1 σ2 σ1' StarN.
+  size induction n.
+
+  inv Sim; zzsimpl.
+    + invc StarN; eauto. zzsimpl.
+      eapply star2_star2n in H4. dcr.
+      edestruct (star2n_reach' H11 H7) as [?|[?|?]]; eauto; subst; dcr. eapply H.
+      * econstructor 1. eapply star2n_plus; eauto. omega. eauto. eauto.
+      * eapply H3; eauto. admit.
+      * subst.
+
+Lemma redc_upto {S} `{StateType S} {S'} `{StateType S'}
+  : (forall r, @redc S _ S' _ (simc r) <3= simc r).
+Proof.
+  intros H1 H2.
+  eapply upto.
+  - unfold redc; hnf; intros.
+    dcr.
+    do  2eexists;  eauto.
+  - unfold redc. intros r UH t σ1 σ2 PR.
+    destruct PR as [σ1' [StarN Sim]].
+    eapply star2_star2n in StarN. destruct StarN as[n StarN].
+    revert dependent r. revert σ1 σ2 σ1' StarN.
+    size induction n.
+    inv Sim; zzsimpl.
+    + invc StarN; eauto. zzsimpl.
+      eapply star2_star2n in H4. dcr.
+      edestruct (star2n_reach' H11 H7) as [?|[?|?]]; eauto; subst; dcr. eapply H.
+      * econstructor 1. eapply star2n_plus; eauto. omega. eauto. eauto.
+      * eapply H3; eauto. admit.
+      * subst.
+
+        eapply H3. Focus 2. eauto. omega. eauto.
+
+
+
+Qed.
+
+
+Lemma redc_simc {S} `{StateType S} {S'} `{StateType S'} (σ1 σ1':S) (σ2 σ2':S') t r
+  : simc r t σ1'  σ2'
+    -> star2 step σ1 nil σ1'
+    -> star2 step σ2 nil σ2'
+    -> simc r t σ1 σ2.
+Proof.
+  intros.
+  eapply redc_upto; hnf; eauto 20.
+Qed.
+
+*)
+
+
+
+Definition sconv {S} `{StateType S} (σ1 σ2:S) :=
+  star2 step σ1 nil σ2 \/ star2 step σ2 nil σ1.
+
+Instance sconv_refl {S} `{StateType S} : Reflexive sconv.
+Proof.
+  hnf; intros; hnf; left; eapply star2_refl.
+Qed.
+
+Instance sconv_sym {S} `{StateType S} : Symmetric sconv.
+Proof.
+  hnf; intros; hnf; firstorder.
+Qed.
+
+Lemma sconv_star2 {S} `{StateType S} (σ1 σ2:S)
+  : star2 step σ1 nil σ2
+    -> sconv σ1 σ2.
+firstorder.
+Qed.
+
+Lemma sconv_plus2 {S} `{StateType S} (σ1 σ2:S)
+  : plus2 step σ1 nil σ2
+    -> sconv σ1 σ2.
+  firstorder using plus2_star2.
+Qed.
+
+Lemma sconv_star2' {S} `{StateType S} (σ1 σ2:S)
+  : star2 step σ1 nil σ2
+    -> sconv σ2 σ1.
+firstorder.
+Qed.
+
+Lemma sconv_plus2' {S} `{StateType S} (σ1 σ2:S)
+  : plus2 step σ1 nil σ2
+    -> sconv σ2 σ1.
+Proof.
+  unfold sconv; intros; eauto using plus2_star2.
+Qed.
+
+Hint Resolve sconv_star2 sconv_plus2 sconv_star2' sconv_plus2'.
+
+Lemma sconv_closed {S} `{StateType S} (σ1 σ2 σ1' σ2':S)
+  : sconv σ1 σ2
+    -> star2 step σ1 nil σ1'
+    -> star2 step σ2 nil σ2'
+    -> sconv σ1' σ2'.
+Proof.
+  unfold sconv; intros; destruct H0; zzsimpl; try zzcases; eauto.
+  edestruct (star2_reach H1 H2); eauto. eapply H.
+  edestruct (star2_reach H1 H2); eauto. eapply H.
+Qed.
+
+Hint Resolve sconv_closed.
+
+Lemma sconv_activated_right  {S} `{StateType S} σ1 σ2
+  : sconv σ1 σ2 -> activated σ2 ->
+    exists σ1', star2 step σ1 nil σ1' /\ activated σ1'.
+Proof.
+  intros. destruct H0.
+  - zzsimpl. eauto.
+  - zzsimpl. eauto using star2.
+Qed.
+
+Ltac fold_conv :=
+  match goal with
+  | [ H : sconv ?σ1 ?σ2, I : star2 step ?σ2 nil ?σ3 |- _ ]
+    => eapply sconv_closed in H; [ clear I | eapply star2_refl | eapply  I]
+  | [ H : sconv ?σ1 ?σ2, I : star2 step ?σ1 nil ?σ3 |- _ ]
+    => eapply sconv_closed in H; [ clear I | eapply  I | eapply star2_refl]
+  end.
+
+
+
+
+Definition g {S} `{StateType S} {S'} `{StateType S'}
+           (r:(simtype -> S -> S' -> Prop)) : simtype -> S -> S' -> Prop :=
+  fun t σ σ' => exists σ1 σ2, simc bot3 t σ σ1 /\
+                      sconv σ1 σ2
+                      /\ r t σ2 σ'.
+
+Lemma g_upto {S} `{StateType S} {S'} `{StateType S'}
+  : (forall r, @g S _ S' _ (simc r) <3= simc r).
+    Proof.
+      intros H1 H2.
+      eapply upto.
+      - unfold g; hnf; intros.
+        destruct IN as [? [? ?]]. dcr.
+        do 2 eexists; split; eauto.
+      - unfold g; intros.
+        destruct PR as [? [? [? [? ?]]]].
+        eapply companion_unfold in H4.
+        + { inv H6.
+          - econstructor 1. eauto. eauto.
+            eapply H3; eauto.
+            do 2 eexists; split; eauto.
+            split; [|eauto].
+            eapply sconv_closed; eauto using plus2_star2.
+          - (* plus step <-> activated *)
+            admit.
+          -
+            zzsimpl. zzcases. zzsimpl.
+        + econstructor 2; eauto using plus2_star2.
+          * intros. unfold upaco3 in *; zzsimpl; eauto 10 using star2_refl.
+          * intros. unfold upaco3 in *; zzsimpl; eauto 10 using star2_refl.
+        + zzsimpl. assert (t = Sim).
+          eapply (@sim_t_Sim_activated t _ _ _ H10 H9 _ _ _ H7); eauto.
+          subst.
+          econstructor 3; eauto using plus2_star2, star2_trans.
+      - (* plus step <-> err *)
+        zzsimpl. zzcases.
+        + pfold. zzsimpl.
+          econstructor 3; eauto; eauto.
+        + eapply plus2_star2 in H4.
+          exploit (star2_trans H4 H2); eauto.
+      - (*  plus step <-> term *)
+        zzsimpl. zzcases.
+        + pfold. zzsimpl.
+          econstructor 4; eauto; eauto.
+        + zzsimpl.
+          destruct (@sim_t_Sim_normal t _ _ _ _ _ _ H9 H8 H14 H7); eauto.
+          * subst.
+            pfold. econstructor 3; eauto using plus2_star2, star2_trans.
+          * pfold. econstructor 4; eauto using plus2_star2, star2_trans.
+            congruence.
+      - (* activated <-> plus step *)
+        pfold. zzsimpl.
+        zzcases. zzsimpl.
+        + unfold upaco3 in *.
+          econstructor 2; eauto using plus2_star2.
+          * intros. zzsimpl; eauto 10 using star2_refl.
+          * intros. zzsimpl; eauto 10 using star2_refl.
+      - (* activated <-> activated *)
+        pfold. zzsimpl.
+        unfold upaco3 in *.
+        econstructor 2; eauto using plus2_star2.
+        * intros. zzsimpl; eauto 10 using star2_refl.
+        * intros. zzsimpl; eauto 10 using star2_refl.
+      - (* activated <-> err *)
+        zzsimpl.
+      - (* activated <-> term *)
+        zzsimpl.
+      - (* term <-> plus step *)
+        case_eq (result σ1'); intros.
+        + pfold. zzsimpl. zzcases.
+          zzsimpl.
+          econstructor 4; eauto. eauto.
+        + zzsimpl.
+          rewrite H4 in H10.
+          destruct (@sim_t_Sim_normal_step _ _ _ _ _ _ _ H10 H9 H15); eauto.
+          * subst.
+            pfold. econstructor 3; eauto. congruence.
+          * destruct H2; dcr.
+            zzsimpl.
+            pfold. econstructor 4; eauto. congruence.
+      - zzsimpl.
+      - (* term <-> err *)
+        zzsimpl.
+        pfold. econstructor 3; eauto. congruence.
+      - (* term <-> term *)
+        zzsimpl.
+        pfold. econstructor 4; eauto. congruence.
+
+
+            + econstructor 1. eauto. eauto.
+              eapply H3; eauto.
+              do 2 eexists; split; eauto.
+          - admit.
+          - admit.
+          - admit.
+          - admit.
+          - admit.
+          - admit.
+          - admit.
+          - admit.
+          - admit.
+          - admit.
+          - admit.
+          - admit.
+          - admit.
+          - admit.
+          - admit.
+          }
+        + {
+            inv H4; inv H6.
+            - zzsimpl. zzcases.
+              + econstructor 1. eauto. eauto.
+              eapply H3; eauto.
+              do 2 eexists; split; eauto.
+              + econstructor 1. eauto. eauto.
+                eapply H3; eauto.
+                do 2 eexists; split; eauto.
+
+          }
+
+    Qed.
+
+Lemma simc_trans_r_right {S} `{StateType S} {S'} `{StateType S'} r t
+       (σ1:S) (σ2a σ2b:S) (σ3:S')
+  : simc bot3 t σ1 σ2a
+    -> (star2 step σ2a nil σ2b \/ star2 step σ2b nil σ2a)
+    -> simc r t σ2b σ3
     -> simc r t σ1 σ3.
 Proof.
-Admitted.
+
+Lemma simc_trans_r_right {S} `{StateType S} {S'} `{StateType S'} r t
+       (σ1:S) (σ2a σ2b:S) (σ3:S')
+  : simc bot3 t σ1 σ2a
+    -> (star2 step σ2a nil σ2b \/ star2 step σ2b nil σ2a)
+    -> simc r t σ2b σ3
+    -> simc r t σ1 σ3.
+Proof.
+  eapply upto.
+  unfold simc.
+  revert σ1 σ2a σ2b σ3. eapply tower_ind; intros.
+  hnf; intros; eauto.
+  intros.
+  assert (sim r t σ2b σ3). admit.
+  eapply simc_sim in H4.
+  eapply companion_fold; eauto using sim_gen_mon.
+  destruct H4.
